I want to switch to master

inference-tool/log_check.py
@@ -16,4 +16,6 @@ for prog in [f for f in os.listdir(root) if os.path.isdir(f"{root}/{f}") and f !
             for run in os.listdir(f"{root}/{prog}/{log}/{config}"):
                 if "testLog.json" not in os.listdir(f"{root}/{prog}/{log}/{config}/{run}"):
                     with open(f"{root}/{prog}/{log}/{config}/{run}/log") as l:
-                        print(l.readline()[26:])
+                        _, s, _, p, _, g, _, o, _, u, _, _, _, df, train, test = l.readline()[26:].split()
+                        base, seed = train.split("/")[2].split("-")
+                        print("sbatch bessemer-run.sh", g, o, u, base, p, seed)
