formal/inference/EFSM_Dot.thy
@@ -9,6 +9,10 @@ theory EFSM_Dot
 imports Inference
 begin
 
+class to_string = fixes toString  :: "'a \<Rightarrow> String.literal" ("toString _" [40] 40)
+
+
+
 fun string_of_digit :: "nat \<Rightarrow> String.literal" where
   "string_of_digit n = (
          if n = 0 then (STR ''0'')
@@ -53,17 +57,9 @@ definition replace_backslash :: "String.literal \<Rightarrow> String.literal" wh
 code_printing
   constant replace_backslash \<rightharpoonup> (Scala) "_.replace(\"\\\\\", \"\\\\\\\\\")"
 
-fun value2dot :: "value \<Rightarrow> String.literal" where
-  "value2dot (value.Str s) = quote + replace_backslash s + quote" |
-  "value2dot (Num n) = show_int n"
-
-fun vname2dot :: "vname \<Rightarrow> String.literal" where
-  "vname2dot (vname.I n) = STR ''i<sub>''+(show_nat (n))+STR ''</sub>''" |
-  "vname2dot (R n) = STR ''r<sub>''+(show_nat n)+STR ''</sub>''"
-
-fun aexp2dot :: "vname aexp \<Rightarrow> String.literal" where
-  "aexp2dot (L v) = value2dot v" |
-  "aexp2dot (V v) = vname2dot v" |
+fun aexp2dot :: "('a::to_string, 'b::to_string) aexp \<Rightarrow> String.literal" where
+  "aexp2dot (L v) = (toString v)" |
+  "aexp2dot (V v) = (toString v)" |
   "aexp2dot (Plus a1 a2) = (aexp2dot a1)+STR '' + ''+(aexp2dot a2)" |
   "aexp2dot (Minus a1 a2) = (aexp2dot a1)+STR '' - ''+(aexp2dot a2)" |
   "aexp2dot (Times a1 a2) = (aexp2dot a1)+STR '' &times; ''+(aexp2dot a2)"
@@ -76,48 +72,64 @@ fun join :: "String.literal list \<Rightarrow> String.literal \<Rightarrow> Stri
 definition show_nats :: "nat list \<Rightarrow> String.literal" where
   "show_nats l = join (map show_nat l) STR '', ''"
 
-fun gexp2dot :: "vname gexp \<Rightarrow> String.literal" where
+fun gexp2dot :: "('a::to_string, 'b::to_string) gexp \<Rightarrow> String.literal" where
   "gexp2dot (GExp.Bc True) = (STR ''True'')" |
   "gexp2dot (GExp.Bc False) = (STR ''False'')" |
   "gexp2dot (GExp.Eq a1 a2) = (aexp2dot a1)+STR '' = ''+(aexp2dot a2)" |
   "gexp2dot (GExp.Gt a1 a2) = (aexp2dot a1)+STR '' &gt; ''+(aexp2dot a2)" |
-  "gexp2dot (GExp.In v l) = (vname2dot v)+STR ''&isin;{''+(join (map value2dot l) STR '', '')+STR ''}''" |
+  "gexp2dot (GExp.In v l) = (toString v)+STR ''&isin;{''+(join (map (\<lambda>x. toString x) l) STR '', '')+STR ''}''" |
   "gexp2dot (Nor g1 g2) = STR ''!(''+(gexp2dot g1)+STR ''&or;''+(gexp2dot g2)+STR '')''"
 
-primrec guards2dot_aux :: "vname gexp list \<Rightarrow> String.literal list" where
+primrec guards2dot_aux :: "('a::to_string, 'b::to_string) gexp list \<Rightarrow> String.literal list" where
   "guards2dot_aux [] = []" |
   "guards2dot_aux (h#t) = (gexp2dot h)#(guards2dot_aux t)"
 
 lemma gexp2dot_aux_code [code]: "guards2dot_aux l = map gexp2dot l"
   by (induct l, simp_all)
 
-primrec updates2dot_aux :: "update_function list \<Rightarrow> String.literal list" where
+instantiation "value" :: to_string begin
+  fun toString_value :: "value \<Rightarrow> String.literal" where
+    "toString_value (value.Str s) = quote + replace_backslash s + quote" |
+    "toString_value (Num n) = show_int n"
+
+  instance by standard
+end
+
+instantiation vname :: to_string begin
+  fun toString_vname :: "vname \<Rightarrow> String.literal" where
+    "toString_vname (vname.I n) = STR ''i<sub>''+(show_nat (n))+STR ''</sub>''" |
+    "toString_vname (R n) = STR ''r<sub>''+(show_nat n)+STR ''</sub>''"
+
+  instance by standard
+end
+
+primrec updates2dot_aux :: "('a::to_string) update_function list \<Rightarrow> String.literal list" where
   "updates2dot_aux [] = []" |
-  "updates2dot_aux (h#t) = ((vname2dot (R (fst h)))+STR '' := ''+(aexp2dot (snd h)))#(updates2dot_aux t)"
+  "updates2dot_aux (h#t) = ((toString (R (fst h)))+STR '' := ''+(aexp2dot (snd h)))#(updates2dot_aux t)"
 
 lemma updates2dot_aux_code [code]:
-  "updates2dot_aux l = map (\<lambda>(r, u). (vname2dot (R r))+STR '' := ''+(aexp2dot u)) l"
+  "updates2dot_aux l = map (\<lambda>(r, u). (toString (R r))+STR '' := ''+(aexp2dot u)) l"
   by (induct l, auto)
 
-primrec outputs2dot :: "output_function list \<Rightarrow> nat \<Rightarrow> String.literal list" where
+primrec outputs2dot :: "('a::to_string) output_function list \<Rightarrow> nat \<Rightarrow> String.literal list" where
   "outputs2dot [] _ = []" |
   "outputs2dot (h#t) n = ((STR ''o<sub>''+(show_nat n))+STR ''</sub> := ''+(aexp2dot h))#(outputs2dot t (n+1))"
 
-fun updates2dot :: "update_function list \<Rightarrow> String.literal" where
+fun updates2dot :: "('a::to_string) update_function list \<Rightarrow> String.literal" where
   "updates2dot [] = (STR '''')" |
   "updates2dot a = STR ''&#91;''+(join (updates2dot_aux a) STR '', '')+STR ''&#93;''"
 
-fun guards2dot :: "vname gexp list \<Rightarrow> String.literal" where
+fun guards2dot :: "('a::to_string, 'b::to_string) gexp list \<Rightarrow> String.literal" where
   "guards2dot [] = (STR '''')" |
   "guards2dot a = STR ''&#91;''+(join (guards2dot_aux a) STR '', '')+STR ''&#93;''"
 
-definition latter2dot :: "transition \<Rightarrow> String.literal" where
+definition latter2dot :: "('a::to_string) transition \<Rightarrow> String.literal" where
   "latter2dot t = (let l = (join (outputs2dot (Outputs t) 1) STR '', '')+(updates2dot (Updates t)) in (if l = (STR '''') then (STR '''') else STR ''/''+l))"
 
-definition transition2dot :: "transition \<Rightarrow> String.literal" where
+definition transition2dot :: "('a::to_string) transition \<Rightarrow> String.literal" where
   "transition2dot t = (Label t)+STR '':''+(show_nat (Arity t))+(guards2dot (Guards t))+(latter2dot t)"
 
-definition efsm2dot :: "transition_matrix \<Rightarrow> String.literal" where
+definition efsm2dot :: "('a::{to_string,linorder}) transition_matrix \<Rightarrow> String.literal" where
   "efsm2dot e = STR ''digraph EFSM{''+newline+
                 STR ''  graph [rankdir=''+quote+(STR ''LR'')+quote+STR '', fontname=''+quote+STR ''Latin Modern Math''+quote+STR ''];''+newline+
                 STR ''  node [color=''+quote+(STR ''black'')+quote+STR '', fillcolor=''+quote+(STR ''white'')+quote+STR '', shape=''+quote+(STR ''circle'')+quote+STR '', style=''+quote+(STR ''filled'')+quote+STR '', fontname=''+quote+STR ''Latin Modern Math''+quote+STR ''];''+newline+
@@ -127,7 +139,7 @@ definition efsm2dot :: "transition_matrix \<Rightarrow> String.literal" where
                   (join ((map (\<lambda>((from, to), t). STR ''  s''+(show_nat from)+STR ''->s''+(show_nat to)+STR ''[label=<<i>''+(transition2dot t)+STR ''</i>>];'') (sorted_list_of_fset e))) newline)+newline+
                 STR ''}''"
 
-definition iefsm2dot :: "iEFSM \<Rightarrow> String.literal" where
+definition iefsm2dot :: "('a::{to_string,linorder}) iEFSM \<Rightarrow> String.literal" where
   "iefsm2dot e = STR ''digraph EFSM{''+newline+
                  STR ''  graph [rankdir=''+quote+(STR ''LR'')+quote+STR '', fontname=''+quote+STR ''Latin Modern Math''+quote+STR ''];''+newline+
                  STR ''  node [color=''+quote+(STR ''black'')+quote+STR '', fillcolor=''+quote+(STR ''white'')+quote+STR '', shape=''+quote+(STR ''circle'')+quote+STR '', style=''+quote+(STR ''filled'')+quote+STR '', fontname=''+quote+STR ''Latin Modern Math''+quote+STR ''];''+newline+
