formal/inference/Inference.thy
@@ -12,51 +12,51 @@ declare One_nat_def [simp del]
 
 subsection\<open>Transition Identifiers\<close>
 
-text\<open>We first need to define the iEFSM data type which assigns each transition a unique identity.
-This is necessary because transitions may not be unique in an EFSM. Assigning transitions a unique
-identifier enables us to look up the origin and destination states of transitions without having to
+text\<open>We first need to define the 'a iEFSM data type which assigns each 'a transition a unique identity.
+This is necessary because 'a transitions may not be unique in an EFSM. Assigning 'a transitions a unique
+identifier enables us to look up the origin and destination states of 'a transitions without having to
 pass them around in the inference functions.\<close>
 
 type_synonym tid = nat
 type_synonym tids = "tid list"
-type_synonym iEFSM = "(tids \<times> (cfstate \<times> cfstate) \<times> transition) fset"
+type_synonym 'a iEFSM = "(tids \<times> (cfstate \<times> cfstate) \<times> 'a transition) fset"
 
-definition origin :: "tids \<Rightarrow> iEFSM \<Rightarrow> nat" where
+definition origin :: "tids \<Rightarrow> 'a iEFSM \<Rightarrow> nat" where
   "origin uid t = fst (fst (snd (fthe_elem (ffilter (\<lambda>x. set uid \<subseteq> set (fst x)) t))))"
 
-definition dest :: "tids \<Rightarrow> iEFSM \<Rightarrow> nat" where
+definition dest :: "tids \<Rightarrow> 'a iEFSM \<Rightarrow> nat" where
   "dest uid t = snd (fst (snd (fthe_elem (ffilter (\<lambda>x. set uid \<subseteq> set (fst x)) t))))"
 
-definition get_by_id :: "iEFSM \<Rightarrow> tid \<Rightarrow> transition" where
+definition get_by_id :: "'a iEFSM \<Rightarrow> tid \<Rightarrow> 'a transition" where
   "get_by_id e uid = (snd \<circ> snd) (fthe_elem (ffilter (\<lambda>(tids, _). uid \<in> set tids) e))"
 
-definition get_by_ids :: "iEFSM \<Rightarrow> tids \<Rightarrow> transition" where
+definition get_by_ids :: "'a iEFSM \<Rightarrow> tids \<Rightarrow> 'a transition" where
   "get_by_ids e uid = (snd \<circ> snd) (fthe_elem (ffilter (\<lambda>(tids, _). set uid \<subseteq> set tids) e))"
 
-definition uids :: "iEFSM \<Rightarrow> nat fset" where
+definition uids :: "'a iEFSM \<Rightarrow> nat fset" where
   "uids e = ffUnion (fimage (fset_of_list \<circ> fst) e)"
 
-definition max_uid :: "iEFSM \<Rightarrow> nat option" where
+definition max_uid :: "'a iEFSM \<Rightarrow> nat option" where
   "max_uid e = (let uids = uids e in if uids = {||} then None else Some (fMax uids))"
 
-definition tm :: "iEFSM \<Rightarrow> transition_matrix" where
+definition tm :: "'a iEFSM \<Rightarrow> 'a transition_matrix" where
   "tm e = fimage snd e"
 
-definition all_regs :: "iEFSM \<Rightarrow> nat set" where
+definition all_regs :: "'a iEFSM \<Rightarrow> nat set" where
   "all_regs e = EFSM.all_regs (tm e)"
 
-definition max_reg :: "iEFSM \<Rightarrow> nat option" where
+definition max_reg :: "'a iEFSM \<Rightarrow> nat option" where
   "max_reg e = EFSM.max_reg (tm e)"
 
 definition "max_reg_total e = (case max_reg e of None \<Rightarrow> 0 | Some r \<Rightarrow> r)"
 
-definition max_output :: "iEFSM \<Rightarrow> nat" where
+definition max_output :: "'a iEFSM \<Rightarrow> nat" where
   "max_output e = EFSM.max_output (tm e)"
 
-definition max_int :: "iEFSM \<Rightarrow> int" where
+definition max_int :: "('a::aexp_value) iEFSM \<Rightarrow> int" where
   "max_int e = EFSM.max_int (tm e)"
 
-definition S :: "iEFSM \<Rightarrow> nat fset" where
+definition S :: "'a iEFSM \<Rightarrow> nat fset" where
   "S m = (fimage (\<lambda>(uid, (s, s'), t). s) m) |\<union>| fimage (\<lambda>(uid, (s, s'), t). s') m"
 
 lemma S_alt: "S t = EFSM.S (tm t)"
@@ -76,25 +76,25 @@ lemma from_in_S:
 subsection\<open>Building the PTA\<close>
 text\<open>The first step in EFSM inference is to construct a PTA from the observed traces in the same way
 as for classical FSM inference. Beginning with the empty EFSM, we iteratively attempt to walk each
-observed trace in the model. When we reach a point where there is no available transition, one is
+observed trace in the model. When we reach a point where there is no available 'a transition, one is
 added. For classical FSMs, this is simply an atomic label. EFSMs deal with data, so we need to add
 guards which test for the observed input values and outputs which produce the observed values.\<close>
 
-primrec make_guard :: "value list \<Rightarrow> nat \<Rightarrow> vname gexp list" where
+primrec make_guard :: "'b list \<Rightarrow> nat \<Rightarrow> (vname, 'b) gexp list" where
 "make_guard [] _ = []" |
 "make_guard (h#t) n = (gexp.Eq (V (vname.I n)) (L h))#(make_guard t (n+1))"
 
-primrec make_outputs :: "value list \<Rightarrow> output_function list" where
+primrec make_outputs :: "'a list \<Rightarrow> 'a output_function list" where
   "make_outputs [] = []" |
   "make_outputs (h#t) = (L h)#(make_outputs t)"
 
-definition max_uid_total :: "iEFSM \<Rightarrow> nat" where
+definition max_uid_total :: "'a iEFSM \<Rightarrow> nat" where
   "max_uid_total e = (case max_uid e of None \<Rightarrow> 0 | Some u \<Rightarrow> u)"
 
-definition add_transition :: "iEFSM \<Rightarrow> cfstate \<Rightarrow> label \<Rightarrow> value list \<Rightarrow> value list \<Rightarrow> iEFSM" where
+definition add_transition :: "'a iEFSM \<Rightarrow> cfstate \<Rightarrow> label \<Rightarrow> 'a list \<Rightarrow> 'a list \<Rightarrow> 'a iEFSM" where
   "add_transition e s label inputs outputs = finsert ([max_uid_total e + 1], (s, (maxS (tm e))+1), \<lparr>Label=label, Arity=length inputs, Guards=(make_guard inputs 0), Outputs=(make_outputs outputs), Updates=[]\<rparr>) e"
 
-fun make_branch :: "iEFSM \<Rightarrow> cfstate \<Rightarrow> registers \<Rightarrow> trace \<Rightarrow> iEFSM" where
+fun make_branch :: "('a::aexp_value) iEFSM \<Rightarrow> cfstate \<Rightarrow> 'a registers \<Rightarrow> 'a trace \<Rightarrow> 'a iEFSM" where
   "make_branch e _ _ [] = e" |
   "make_branch e s r ((label, inputs, outputs)#t) =
     (case (step (tm e) s r label inputs) of
@@ -107,7 +107,7 @@ fun make_branch :: "iEFSM \<Rightarrow> cfstate \<Rightarrow> registers \<Righta
           make_branch (add_transition e s label inputs outputs) ((maxS (tm e))+1) r t
     )"
 
-primrec make_pta_aux :: "log \<Rightarrow> iEFSM \<Rightarrow> iEFSM" where
+primrec make_pta_aux :: "('a::{aexp_value,order}) log \<Rightarrow> 'a iEFSM \<Rightarrow> 'a iEFSM" where
   "make_pta_aux [] e = e" |
   "make_pta_aux (h#t) e = make_pta_aux t (make_branch e 0 <> h)"
 
@@ -119,26 +119,26 @@ lemma make_pta_aux_fold [code]:
 
 subsection\<open>Integrating Heuristics\<close>
 text\<open>A key contribution of the inference technique presented in \cite{foster2019} is the ability to
-introduce \emph{internal variables} to the model to generalise behaviours and allow transitions to
+introduce \emph{internal variables} to the model to generalise behaviours and allow 'a transitions to
 be merged. This is done by providing the inference technique with a set of \emph{heuristics}. The
 aim here is not to create a ``one size fits all'' magic oracle, rather to recognise particular
 \emph{data usage patterns} which can be abstracted.\<close>
 
-type_synonym update_modifier = "tids \<Rightarrow> tids \<Rightarrow> cfstate \<Rightarrow> iEFSM \<Rightarrow> iEFSM \<Rightarrow> iEFSM \<Rightarrow> (transition_matrix \<Rightarrow> bool) \<Rightarrow> iEFSM option"
+type_synonym 'a update_modifier = "tids \<Rightarrow> tids \<Rightarrow> cfstate \<Rightarrow> 'a iEFSM \<Rightarrow> 'a iEFSM \<Rightarrow> 'a iEFSM \<Rightarrow> ('a transition_matrix \<Rightarrow> bool) \<Rightarrow> 'a iEFSM option"
 
-definition null_modifier :: update_modifier where
+definition null_modifier :: "'a update_modifier" where
   "null_modifier f _ _ _ _ _ _ = None"
 
-definition replace_transition :: "iEFSM \<Rightarrow> tids \<Rightarrow> transition \<Rightarrow> iEFSM" where
+definition replace_transition :: "'a iEFSM \<Rightarrow> tids \<Rightarrow> 'a transition \<Rightarrow> 'a iEFSM" where
   "replace_transition e uid new = (fimage (\<lambda>(uids, (from, to), t). if set uid \<subseteq> set uids then (uids, (from, to), new) else (uids, (from, to), t)) e)"
 
-definition replace_all :: "iEFSM \<Rightarrow> tids list \<Rightarrow> transition \<Rightarrow> iEFSM" where
+definition replace_all :: "'a iEFSM \<Rightarrow> tids list \<Rightarrow> 'a transition \<Rightarrow> 'a iEFSM" where
   "replace_all e ids new = fold (\<lambda>id acc. replace_transition acc id new) ids e"
 
-definition replace_transitions :: "iEFSM \<Rightarrow> (tids \<times> transition) list \<Rightarrow> iEFSM" where
+definition replace_transitions :: "'a iEFSM \<Rightarrow> (tids \<times> 'a transition) list \<Rightarrow> 'a iEFSM" where
   "replace_transitions e ts = fold (\<lambda>(uid, new) acc. replace_transition acc uid new) ts e"
 
-primrec try_heuristics_check :: "(transition_matrix \<Rightarrow> bool) \<Rightarrow> update_modifier list \<Rightarrow> update_modifier" where
+primrec try_heuristics_check :: "('a transition_matrix \<Rightarrow> bool) \<Rightarrow> 'a update_modifier list \<Rightarrow> 'a update_modifier" where
   "try_heuristics_check _ [] = null_modifier" |
   "try_heuristics_check check (h#t) = (\<lambda>a b c d e f ch.
     case h a b c d e f ch of
@@ -176,12 +176,12 @@ instance
 end
 
 type_synonym scoreboard = "score fset"
-type_synonym strategy = "tids \<Rightarrow> tids \<Rightarrow> iEFSM \<Rightarrow> nat"
+type_synonym 'a strategy = "tids \<Rightarrow> tids \<Rightarrow> 'a iEFSM \<Rightarrow> nat"
 
-definition outgoing_transitions :: "cfstate \<Rightarrow> iEFSM \<Rightarrow> (cfstate \<times> transition \<times> tids) fset" where
+definition outgoing_transitions :: "cfstate \<Rightarrow> 'a iEFSM \<Rightarrow> (cfstate \<times> 'a transition \<times> tids) fset" where
   "outgoing_transitions s e = fimage (\<lambda>(uid, (from, to), t'). (to, t', uid)) ((ffilter (\<lambda>(uid, (origin, dest), t). origin = s)) e)"
 
-primrec paths_of_length :: "nat \<Rightarrow> iEFSM \<Rightarrow> cfstate \<Rightarrow> tids list fset" where
+primrec paths_of_length :: "nat \<Rightarrow> 'a iEFSM \<Rightarrow> cfstate \<Rightarrow> tids list fset" where
   "paths_of_length 0 _ _ = {|[]|}" |
   "paths_of_length (Suc m) e s = (
     let
@@ -201,7 +201,7 @@ lemma paths_of_length_1: "paths_of_length 1 e s = fimage (\<lambda>(d, t, id). [
   apply (simp add: ffilter_def ffUnion_def fBall_def Abs_fset_inverse fset_both_sides)
   by force
 
-fun step_score :: "(tids \<times> tids) list \<Rightarrow> iEFSM \<Rightarrow> strategy \<Rightarrow> nat" where
+fun step_score :: "(tids \<times> tids) list \<Rightarrow> 'a iEFSM \<Rightarrow> 'a strategy \<Rightarrow> nat" where
   "step_score [] _ _ = 0" |
   "step_score ((id1, id2)#t) e s = (
     let score = s id1 id2 e in
@@ -228,7 +228,7 @@ next
     by (simp add: Let_def)
 qed
 
-definition score_from_list :: "tids list fset \<Rightarrow> tids list fset \<Rightarrow> iEFSM \<Rightarrow> strategy \<Rightarrow> nat" where
+definition score_from_list :: "tids list fset \<Rightarrow> tids list fset \<Rightarrow> 'a iEFSM \<Rightarrow> 'a strategy \<Rightarrow> nat" where
   "score_from_list P1 P2 e s = (
     let
       pairs = fimage (\<lambda>(l1, l2). zip l1 l2) (P1 |\<times>| P2);
@@ -237,7 +237,7 @@ definition score_from_list :: "tids list fset \<Rightarrow> tids list fset \<Rig
     fSum scored_pairs
   )"
 
-definition k_score :: "nat \<Rightarrow> iEFSM \<Rightarrow> strategy \<Rightarrow> scoreboard" where
+definition k_score :: "nat \<Rightarrow> 'a iEFSM \<Rightarrow> 'a strategy \<Rightarrow> scoreboard" where
   "k_score k e strat = (
     let
       states = S e;
@@ -248,7 +248,7 @@ definition k_score :: "nat \<Rightarrow> iEFSM \<Rightarrow> strategy \<Rightarr
     ffilter (\<lambda>x. Score x > 0) scores
 )"
 
-definition score_state_pair :: "strategy \<Rightarrow> iEFSM \<Rightarrow> cfstate \<Rightarrow> cfstate \<Rightarrow> nat" where
+definition score_state_pair :: "'a strategy \<Rightarrow> 'a iEFSM \<Rightarrow> cfstate \<Rightarrow> cfstate \<Rightarrow> nat" where
   "score_state_pair strat e s1 s2 = (
     let
       T1 = outgoing_transitions s1 e;
@@ -257,7 +257,7 @@ definition score_state_pair :: "strategy \<Rightarrow> iEFSM \<Rightarrow> cfsta
       fSum (fimage (\<lambda>((_, _, t1), (_, _, t2)). strat t1 t2 e) (T1 |\<times>| T2))
   )"
 
-definition score_1 :: "iEFSM \<Rightarrow> strategy \<Rightarrow> scoreboard" where
+definition score_1 :: "'a iEFSM \<Rightarrow> 'a strategy \<Rightarrow> scoreboard" where
   "score_1 e strat = (
     let
       states = S e;
@@ -303,7 +303,7 @@ fun bool2nat :: "bool \<Rightarrow> nat" where
   "bool2nat True = 1" |
   "bool2nat False = 0"
 
-definition score_transitions :: "transition \<Rightarrow> transition \<Rightarrow> nat" where
+definition score_transitions :: "'a transition \<Rightarrow> 'a transition \<Rightarrow> nat" where
   "score_transitions t1 t2 = (
     if Label t1 = Label t2 \<and> Arity t1 = Arity t2 \<and> length (Outputs t1) = length (Outputs t2) then
       1 + bool2nat (t1 = t2) + card ((set (Guards t2)) \<inter> (set (Guards t2))) + card ((set (Updates t2)) \<inter> (set (Updates t2))) + card ((set (Outputs t2)) \<inter> (set (Outputs t2)))
@@ -312,25 +312,25 @@ definition score_transitions :: "transition \<Rightarrow> transition \<Rightarro
   )"
 
 subsection\<open>Direct Subsumption\<close>
-text\<open>When merging EFSM transitions, one must \emph{account for} the behaviour of the other. The
+text\<open>When merging EFSM 'a transitions, one must \emph{account for} the behaviour of the other. The
 \emph{subsumption in context} relation formalises the intuition that, in certain contexts, a
 transition $t_2$ reproduces the behaviour of, and updates the data state in a manner consistent
-with, another transition $t_1$, meaning that $t_2$ can be used in place of $t_1$ with no observable
+with, another 'a transition $t_1$, meaning that $t_2$ can be used in place of $t_1$ with no observable
 difference in behaviour.
 
 The subsumption in context relation requires us to supply a context in which to test subsumption,
 but there is a problem when we try to apply this to inference: Which context should we use? The
-\emph{direct subsumption} relation works at EFSM level to determine when and whether one transition
+\emph{direct subsumption} relation works at EFSM level to determine when and whether one 'a transition
 is able to account for the behaviour of another such that we can use one in place of another without
 adversely effecting observable behaviour.\<close>
 
-definition directly_subsumes :: "iEFSM \<Rightarrow> iEFSM \<Rightarrow> cfstate \<Rightarrow> cfstate \<Rightarrow> transition \<Rightarrow> transition \<Rightarrow> bool" where
+definition directly_subsumes :: "('a::{order,aexp_value}) iEFSM \<Rightarrow> 'a iEFSM \<Rightarrow> cfstate \<Rightarrow> cfstate \<Rightarrow> 'a transition \<Rightarrow> 'a transition \<Rightarrow> bool" where
   "directly_subsumes e1 e2 s s' t1 t2 \<equiv> (\<forall>p. recognises (tm e1) p \<and> gets_us_to s (tm e1) 0 <>  p \<longrightarrow>
                                              recognises (tm e2) p \<and> gets_us_to s' (tm e2) 0 <>  p \<longrightarrow>
                                              (\<forall>c. anterior_context (tm e2) p = Some c \<longrightarrow> subsumes t1 c t2)) \<and>
                                          (\<exists>c. subsumes t1 c t2)"
 
-lemma directly_subsumes_self: "directly_subsumes e1 e2 s s' t t"
+lemma directly_subsumes_reflexive: "directly_subsumes e1 e2 s s' t t"
   apply (simp add: directly_subsumes_def)
   by (simp add: transition_subsumes_self)
 
@@ -352,7 +352,7 @@ lemma cant_directly_subsume:
   "(\<And>c. \<not> subsumes t c t') \<Longrightarrow> \<not> directly_subsumes m m' s s' t t'"
   by (simp add: directly_subsumes_def)
 
-definition insert_transition :: "tids \<Rightarrow> cfstate \<Rightarrow> cfstate \<Rightarrow> transition \<Rightarrow> iEFSM \<Rightarrow> iEFSM" where
+definition insert_transition :: "tids \<Rightarrow> cfstate \<Rightarrow> cfstate \<Rightarrow> 'a transition \<Rightarrow> 'a iEFSM \<Rightarrow> 'a iEFSM" where
   "insert_transition uid from to t e = (
     if \<nexists>(uid, (from', to'), t') |\<in>| e. from = from' \<and> to = to' \<and> t = t' then
       finsert (uid, (from, to), t) e
@@ -375,10 +375,7 @@ lemma guard_implication: "Label t1 = Label t2 \<Longrightarrow>
   unfolding can_take_transition_def can_take_def
   using can_take_transition_def can_take_def posterior_def posterior_separate_def can_take_def by auto
 
-definition gexp_implies :: "'a gexp \<Rightarrow> 'a gexp \<Rightarrow> bool" where
-  "gexp_implies g1 g2 = (\<forall>s. gval g1 s = true \<longrightarrow> gval g2 s = true)"
-
-definition guard_implication_subsumption :: "transition \<Rightarrow> transition \<Rightarrow> bool" where
+definition guard_implication_subsumption :: "('a::aexp_value) transition \<Rightarrow> 'a transition \<Rightarrow> bool" where
   "guard_implication_subsumption t1 t2 = (
     Label t1 = Label t2 \<and>
     Arity t1 = Arity t2 \<and>
@@ -392,14 +389,16 @@ lemma guard_implication_subsumption:
   apply (rule subsumes_in_all_contexts_directly_subsumes)
   apply (rule subsumption)
   unfolding guard_implication_subsumption_def can_take_transition_def can_take_def
-  using gexp_implies_def apply_guards_fold can_take_transition_def can_take_def
-        posterior_def posterior_separate_def can_take_def by auto
+     apply simp
+    apply (simp add: fold_apply_guards gexp_implies_def)
+   apply simp
+  by simp
 
 subsection\<open>Merging States\<close>
-definition merge_states_aux :: "nat \<Rightarrow> nat \<Rightarrow> iEFSM \<Rightarrow> iEFSM" where
+definition merge_states_aux :: "nat \<Rightarrow> nat \<Rightarrow> 'a iEFSM \<Rightarrow> 'a iEFSM" where
   "merge_states_aux s1 s2 e = fimage (\<lambda>(uid, (origin, dest), t). (uid, (if origin = s1 then s2 else origin , if dest = s1 then s2 else dest), t)) e"
 
-definition merge_states :: "nat \<Rightarrow> nat \<Rightarrow> iEFSM \<Rightarrow> iEFSM" where
+definition merge_states :: "nat \<Rightarrow> nat \<Rightarrow> 'a iEFSM \<Rightarrow> 'a iEFSM" where
   "merge_states x y t = (if x > y then merge_states_aux x y t else merge_states_aux y x t)"
 
 lemma merge_states_symmetry: "merge_states x y t = merge_states y x t"
@@ -415,15 +414,15 @@ lemma merge_states_self_simp [code]:
   by force
 
 subsection\<open>Resolving Nondeterminism\<close>
-text\<open>Because EFSM transitions are not simply atomic actions, duplicated behaviours cannot be
-resolved into a single transition by simply merging destination states, as it can in classical FSM
+text\<open>Because EFSM 'a transitions are not simply atomic actions, duplicated behaviours cannot be
+resolved into a single 'a transition by simply merging destination states, as it can in classical FSM
 inference. It is now possible for attempts to resolve the nondeterminism introduced by merging
 states to fail, meaning that two states which initially seemed compatible cannot actually be merged.
 This is not the case in classical FSM inference.\<close>
 
-type_synonym nondeterministic_pair = "(cfstate \<times> (cfstate \<times> cfstate) \<times> ((transition \<times> tids) \<times> (transition \<times> tids)))"
+type_synonym 'a nondeterministic_pair = "(cfstate \<times> (cfstate \<times> cfstate) \<times> (('a transition \<times> tids) \<times> ('a transition \<times> tids)))"
 
-definition state_nondeterminism :: "nat \<Rightarrow> (cfstate \<times> transition \<times> tids) fset \<Rightarrow> nondeterministic_pair fset" where
+definition state_nondeterminism :: "nat \<Rightarrow> (cfstate \<times> 'a transition \<times> tids) fset \<Rightarrow> 'a nondeterministic_pair fset" where
   "state_nondeterminism og nt = (if size nt < 2 then {||} else ffUnion (fimage (\<lambda>x. let (dest, t) = x in fimage (\<lambda>y. let (dest', t') = y in (og, (dest, dest'), (t, t'))) (nt - {|x|})) nt))"
 
 lemma state_nondeterminism_empty [simp]: "state_nondeterminism a {||} = {||}"
@@ -432,53 +431,53 @@ lemma state_nondeterminism_empty [simp]: "state_nondeterminism a {||} = {||}"
 lemma state_nondeterminism_singledestn [simp]: "state_nondeterminism a {|x|} = {||}"
   by (simp add: state_nondeterminism_def ffilter_def Set.filter_def)
 
-(* For each state, get its outgoing transitions and see if there's any nondeterminism there *)
-definition nondeterministic_pairs :: "iEFSM \<Rightarrow> nondeterministic_pair fset" where
+(* For each state, get its outgoing 'a transitions and see if there's any nondeterminism there *)
+definition nondeterministic_pairs :: "('a::aexp_value) iEFSM \<Rightarrow> 'a nondeterministic_pair fset" where
   "nondeterministic_pairs t = ffilter (\<lambda>(_, _, (t, _), (t', _)). Label t = Label t' \<and> Arity t = Arity t' \<and> choice t t') (ffUnion (fimage (\<lambda>s. state_nondeterminism s (outgoing_transitions s t)) (S t)))"
 
-definition nondeterministic_pairs_labar_dest :: "iEFSM \<Rightarrow> nondeterministic_pair fset" where
+definition nondeterministic_pairs_labar_dest :: "('a::aexp_value) iEFSM \<Rightarrow> 'a nondeterministic_pair fset" where
   "nondeterministic_pairs_labar_dest t = ffilter
      (\<lambda>(_, (d, d'), (t, _), (t', _)).
       Label t = Label t' \<and> Arity t = Arity t' \<and> (choice t t' \<or> (Outputs t = Outputs t' \<and> d = d')))
      (ffUnion (fimage (\<lambda>s. state_nondeterminism s (outgoing_transitions s t)) (S t)))"
 
-definition nondeterministic_pairs_labar :: "iEFSM \<Rightarrow> nondeterministic_pair fset" where
+definition nondeterministic_pairs_labar :: "('a::aexp_value) iEFSM \<Rightarrow> 'a nondeterministic_pair fset" where
   "nondeterministic_pairs_labar t = ffilter
      (\<lambda>(_, (d, d'), (t, _), (t', _)).
       Label t = Label t' \<and> Arity t = Arity t' \<and> (choice t t' \<or> Outputs t = Outputs t'))
      (ffUnion (fimage (\<lambda>s. state_nondeterminism s (outgoing_transitions s t)) (S t)))"
 
-definition deterministic :: "iEFSM \<Rightarrow> (iEFSM \<Rightarrow> nondeterministic_pair fset) \<Rightarrow> bool" where
+definition deterministic :: "'a iEFSM \<Rightarrow> ('a iEFSM \<Rightarrow> 'a nondeterministic_pair fset) \<Rightarrow> bool" where
   "deterministic t np = (np t = {||})"
 
-definition nondeterministic :: "iEFSM \<Rightarrow> (iEFSM \<Rightarrow> nondeterministic_pair fset) \<Rightarrow> bool" where
+definition nondeterministic :: "'a iEFSM \<Rightarrow> ('a iEFSM \<Rightarrow> 'a nondeterministic_pair fset) \<Rightarrow> bool" where
   "nondeterministic t np = (\<not> deterministic t np)"
 
-definition make_distinct :: "iEFSM \<Rightarrow> iEFSM" where
+definition make_distinct :: "('a::linorder) iEFSM \<Rightarrow> 'a iEFSM" where
   "make_distinct e = ffold_ord (\<lambda>(uid, (from, to), t) acc. insert_transition uid from to t acc) e {||}"
 
-\<comment> \<open>When we replace one transition with another, we need to merge their uids to keep track of which\<close>
+\<comment> \<open>When we replace one 'a transition with another, we need to merge their uids to keep track of which\<close>
 \<comment> \<open>transition accounts for which action in the original traces                                     \<close>
-definition merge_transitions_aux :: "iEFSM \<Rightarrow> tids \<Rightarrow> tids \<Rightarrow> iEFSM" where
+definition merge_transitions_aux :: "('a::linorder) iEFSM \<Rightarrow> tids \<Rightarrow> tids \<Rightarrow> 'a iEFSM" where
   "merge_transitions_aux e oldID newID = (let
     (uids1, (origin, dest), old) = fthe_elem (ffilter (\<lambda>(uids, _). oldID = uids) e);
     (uids2, (origin, dest), new) = fthe_elem (ffilter (\<lambda>(uids, _). newID = uids) e) in
     make_distinct (finsert (List.union uids1 uids2, (origin, dest), new) (e - {|(uids1, (origin, dest), old), (uids2, (origin, dest), new)|}))
   )"
 
-(* merge_transitions - Try dest merge transitions t\<^sub>1 and t\<^sub>2 dest help resolve nondeterminism in
-                       newEFSM. If either subsumes the other directly then the subsumed transition
+(* merge_transitions - Try dest merge 'a transitions t\<^sub>1 and t\<^sub>2 dest help resolve nondeterminism in
+                       newEFSM. If either subsumes the other directly then the subsumed 'a transition
                        can simply be replaced with the subsuming one, else we try dest apply the
                        modifier function dest resolve nondeterminism that way.                    *)
 (* @param oldEFSM   - the EFSM before merging the states which caused the nondeterminism          *)
 (* @param preDestMerge   - the EFSM after merging the states which caused the nondeterminism      *)
 (* @param newEFSM   - the current EFSM with nondeterminism                                        *)
-(* @param t\<^sub>1        - a transition dest be merged with t\<^sub>2                                         *)
+(* @param t\<^sub>1        - a 'a transition dest be merged with t\<^sub>2                                         *)
 (* @param u\<^sub>1        - the unique identifier of t\<^sub>1                                                 *)
-(* @param t\<^sub>2        - a transition dest be merged with t\<^sub>1                                         *)
+(* @param t\<^sub>2        - a 'a transition dest be merged with t\<^sub>1                                         *)
 (* @param u\<^sub>2        - the unique identifier of t\<^sub>2                                                 *)
-(* @param modifier  - an update modifier function which tries dest generalise transitions         *)
-definition merge_transitions :: "(cfstate \<times> cfstate) set \<Rightarrow> iEFSM \<Rightarrow> iEFSM \<Rightarrow> iEFSM \<Rightarrow> transition \<Rightarrow> tids \<Rightarrow> transition \<Rightarrow> tids \<Rightarrow> update_modifier \<Rightarrow> (transition_matrix \<Rightarrow> bool) \<Rightarrow> iEFSM option" where
+(* @param modifier  - an update modifier function which tries dest generalise 'a transitions         *)
+definition merge_transitions :: "(cfstate \<times> cfstate) set \<Rightarrow> ('a::{aexp_value, linorder}) iEFSM \<Rightarrow> 'a iEFSM \<Rightarrow> 'a iEFSM \<Rightarrow> 'a transition \<Rightarrow> tids \<Rightarrow> 'a transition \<Rightarrow> tids \<Rightarrow> 'a update_modifier \<Rightarrow> ('a transition_matrix \<Rightarrow> bool) \<Rightarrow> 'a iEFSM option" where
   "merge_transitions failedMerges oldEFSM preDestMerge destMerge t\<^sub>1 u\<^sub>1 t\<^sub>2 u\<^sub>2 modifier check = (
      if \<forall>id \<in> set u\<^sub>1. directly_subsumes oldEFSM destMerge (origin [id] oldEFSM) (origin u\<^sub>1 destMerge) t\<^sub>2 t\<^sub>1 then
        \<comment> \<open>Replace t1 with t2\<close>
@@ -492,28 +491,28 @@ definition merge_transitions :: "(cfstate \<times> cfstate) set \<Rightarrow> iE
           Some e \<Rightarrow> Some (make_distinct e)
    )"
 
-definition outgoing_transitions_from :: "iEFSM \<Rightarrow> cfstate \<Rightarrow> transition fset" where
+definition outgoing_transitions_from :: "'a iEFSM \<Rightarrow> cfstate \<Rightarrow> 'a transition fset" where
   "outgoing_transitions_from e s = fimage (\<lambda>(_, _, t). t) (ffilter (\<lambda>(_, (orig, _), _). orig = s) e)"
 
-definition order_nondeterministic_pairs :: "nondeterministic_pair fset \<Rightarrow> nondeterministic_pair list" where
+definition order_nondeterministic_pairs :: "('a::linorder) nondeterministic_pair fset \<Rightarrow> 'a nondeterministic_pair list" where
   "order_nondeterministic_pairs s = map snd (sorted_list_of_fset (fimage (\<lambda>s. let (_, _, (t1, _), (t2, _)) = s in (score_transitions t1 t2, s)) s))"
 
-(* resolve_nondeterminism - tries dest resolve nondeterminism in a given iEFSM                      *)
+(* resolve_nondeterminism - tries dest resolve nondeterminism in a given 'a iEFSM                      *)
 (* @param ((from, (dest\<^sub>1, dest\<^sub>2), ((t\<^sub>1, u\<^sub>1), (t\<^sub>2, u\<^sub>2)))#ss) - a list of nondeterministic pairs where
           from - nat - the state from which t\<^sub>1 and t\<^sub>2 eminate
           dest\<^sub>1  - nat - the destination state of t\<^sub>1
           dest\<^sub>2  - nat - the destination state of t\<^sub>2
-          t\<^sub>1   - transition - a transition dest be merged with t\<^sub>2
-          t\<^sub>2   - transition - a transition dest be merged with t\<^sub>1
+          t\<^sub>1   - 'a transition - a 'a transition dest be merged with t\<^sub>2
+          t\<^sub>2   - 'a transition - a 'a transition dest be merged with t\<^sub>1
           u\<^sub>1   - nat - the unique identifier of t\<^sub>1
           u\<^sub>2   - nat - the unique identifier of t\<^sub>2
           ss   - list - the rest of the list                                                      *)
 (* @param oldEFSM - the EFSM before merging the states which caused the nondeterminism            *)
 (* @param newEFSM - the current EFSM with nondeterminism                                          *)
-(* @param m       - an update modifier function which tries dest generalise transitions             *)
+(* @param m       - an update modifier function which tries dest generalise 'a transitions             *)
 (* @param check - a function which takes an EFSM and returns a bool dest ensure that certain
-                  properties hold in the new iEFSM                                                *)
-function resolve_nondeterminism :: "(cfstate \<times> cfstate) set \<Rightarrow> nondeterministic_pair list \<Rightarrow> iEFSM \<Rightarrow> iEFSM \<Rightarrow> update_modifier \<Rightarrow> (transition_matrix \<Rightarrow> bool) \<Rightarrow> (iEFSM \<Rightarrow> nondeterministic_pair fset) \<Rightarrow> (iEFSM option \<times> (cfstate \<times> cfstate) set)" where
+                  properties hold in the new 'a iEFSM                                                *)
+function resolve_nondeterminism :: "(cfstate \<times> cfstate) set \<Rightarrow> ('a::{aexp_value,linorder}) nondeterministic_pair list \<Rightarrow> 'a iEFSM \<Rightarrow> 'a iEFSM \<Rightarrow> 'a update_modifier \<Rightarrow> ('a transition_matrix \<Rightarrow> bool) \<Rightarrow> ('a iEFSM \<Rightarrow> 'a nondeterministic_pair fset) \<Rightarrow> ('a iEFSM option \<times> (cfstate \<times> cfstate) set)" where
   "resolve_nondeterminism failedMerges [] _ newEFSM _ check np = (
       if deterministic newEFSM np \<and> check (tm newEFSM) then Some newEFSM else None, failedMerges
   )" |
@@ -543,14 +542,14 @@ termination
 
 subsection\<open>EFSM Inference\<close>
 
-(* Merge - tries dest merge two states in a given iEFSM and resolve the resulting nondeterminism  *)
-(* @param e     - an iEFSM                                                                        *)
+(* Merge - tries dest merge two states in a given 'a iEFSM and resolve the resulting nondeterminism  *)
+(* @param e     - an 'a iEFSM                                                                        *)
 (* @param s1    - a state dest be merged with s2                                                  *)
 (* @param s2    - a state dest be merged with s1                                                  *)
-(* @param m     - an update modifier function which tries dest generalise transitions             *)
+(* @param m     - an update modifier function which tries dest generalise 'a transitions             *)
 (* @param check - a function which takes an EFSM and returns a bool dest ensure that certain
-                  properties hold in the new iEFSM                                                *)
-definition merge :: "(cfstate \<times> cfstate) set \<Rightarrow> iEFSM \<Rightarrow> nat \<Rightarrow> nat \<Rightarrow> update_modifier \<Rightarrow> (transition_matrix \<Rightarrow> bool) \<Rightarrow> (iEFSM \<Rightarrow> nondeterministic_pair fset) \<Rightarrow> (iEFSM option \<times> (cfstate \<times> cfstate) set)" where
+                  properties hold in the new 'a iEFSM                                                *)
+definition merge :: "(cfstate \<times> cfstate) set \<Rightarrow> ('a::{linorder,aexp_value}) iEFSM \<Rightarrow> nat \<Rightarrow> nat \<Rightarrow> 'a update_modifier \<Rightarrow> ('a transition_matrix \<Rightarrow> bool) \<Rightarrow> ('a iEFSM \<Rightarrow> 'a nondeterministic_pair fset) \<Rightarrow> ('a iEFSM option \<times> (cfstate \<times> cfstate) set)" where
   "merge failedMerges e s\<^sub>1 s\<^sub>2 m check np = (
     if s\<^sub>1 = s\<^sub>2 \<or> (s\<^sub>1, s\<^sub>2) \<in> failedMerges \<or> (s\<^sub>2, s\<^sub>1) \<in> failedMerges then
       (None, failedMerges)
@@ -560,12 +559,12 @@ definition merge :: "(cfstate \<times> cfstate) set \<Rightarrow> iEFSM \<Righta
   )"
 
 (* inference_step - attempt dest carry out a single step of the inference process by merging the  *)
-(* @param e - an iEFSM dest be generalised                                                        *)
+(* @param e - an 'a iEFSM dest be generalised                                                        *)
 (* @param ((s, s1, s2)#t) - a list of triples of the form (score, state, state) dest be merged    *)
-(* @param m     - an update modifier function which tries dest generalise transitions             *)
+(* @param m     - an update modifier function which tries dest generalise 'a transitions             *)
 (* @param check - a function which takes an EFSM and returns a bool dest ensure that certain
-                  properties hold in the new iEFSM                                                *)
-function inference_step :: "(cfstate \<times> cfstate) set \<Rightarrow> iEFSM \<Rightarrow> score fset \<Rightarrow> update_modifier \<Rightarrow> (transition_matrix \<Rightarrow> bool) \<Rightarrow> (iEFSM \<Rightarrow> nondeterministic_pair fset) \<Rightarrow> (iEFSM option \<times> (cfstate \<times> cfstate) set)" where
+                  properties hold in the new 'a iEFSM                                                *)
+function inference_step :: "(cfstate \<times> cfstate) set \<Rightarrow> ('a::{linorder,aexp_value}) iEFSM \<Rightarrow> score fset \<Rightarrow> 'a update_modifier \<Rightarrow> ('a transition_matrix \<Rightarrow> bool) \<Rightarrow> ('a iEFSM \<Rightarrow> 'a nondeterministic_pair fset) \<Rightarrow> ('a iEFSM option \<times> (cfstate \<times> cfstate) set)" where
   "inference_step failedMerges e s m check np = (
      if s = {||} then (None, failedMerges) else
      let
@@ -582,13 +581,13 @@ termination
    apply simp
   by (simp add: card_minus_fMin)
 
-(* Takes an iEFSM and iterates inference_step until no further states can be successfully merged  *)
-(* @param e - an iEFSM dest be generalised                                                        *)
-(* @param r - a strategy dest identify and prioritise pairs of states dest merge                  *)
-(* @param m     - an update modifier function which tries dest generalise transitions             *)
+(* Takes an 'a iEFSM and iterates inference_step until no further states can be successfully merged  *)
+(* @param e - an 'a iEFSM dest be generalised                                                        *)
+(* @param r - a 'a strategy dest identify and prioritise pairs of states dest merge                  *)
+(* @param m     - an update modifier function which tries dest generalise 'a transitions             *)
 (* @param check - a function which takes an EFSM and returns a bool dest ensure that certain
-                  properties hold in the new iEFSM                                                *)
-function infer :: "(cfstate \<times> cfstate) set \<Rightarrow> nat \<Rightarrow> iEFSM \<Rightarrow> strategy \<Rightarrow> update_modifier \<Rightarrow> (transition_matrix \<Rightarrow> bool) \<Rightarrow> (iEFSM \<Rightarrow> nondeterministic_pair fset) \<Rightarrow> iEFSM" where
+                  properties hold in the new 'a iEFSM                                                *)
+function infer :: "(cfstate \<times> cfstate) set \<Rightarrow> nat \<Rightarrow> ('a::{linorder,aexp_value}) iEFSM \<Rightarrow> 'a strategy \<Rightarrow> 'a update_modifier \<Rightarrow> ('a transition_matrix \<Rightarrow> bool) \<Rightarrow> ('a iEFSM \<Rightarrow> 'a nondeterministic_pair fset) \<Rightarrow> 'a iEFSM" where
   "infer failedMerges k e r m check np = (
     let scores = if k = 1 then score_1 e r else (k_score k e r) in
     case inference_step failedMerges e (ffilter (\<lambda>s. (S1 s, S2 s) \<notin> failedMerges \<and> (S2 s, S1 s) \<notin> failedMerges) scores) m check np of
@@ -601,11 +600,11 @@ termination
    apply simp
   by (metis (no_types, lifting) case_prod_conv measures_less size_fsubset)
 
-fun get_ints :: "trace \<Rightarrow> int list" where
+fun get_ints :: "('a::aexp_value) trace \<Rightarrow> int list" where
   "get_ints [] = []" |
-  "get_ints ((_, inputs, outputs)#t) = (map (\<lambda>x. case x of Num n \<Rightarrow> n) (filter is_Num (inputs@outputs)))"
+  "get_ints ((_, inputs, outputs)#t) = (map (\<lambda>x. getNum x) (filter (\<lambda> x. isNum x) (inputs@outputs)))"
 
-definition learn :: "nat \<Rightarrow> iEFSM \<Rightarrow> log \<Rightarrow> strategy \<Rightarrow> update_modifier \<Rightarrow> (iEFSM \<Rightarrow> nondeterministic_pair fset) \<Rightarrow> iEFSM" where
+definition learn :: "nat \<Rightarrow> ('a::{aexp_value,linorder}) iEFSM \<Rightarrow> 'a log \<Rightarrow> 'a strategy \<Rightarrow> 'a update_modifier \<Rightarrow> ('a iEFSM \<Rightarrow> 'a nondeterministic_pair fset) \<Rightarrow> 'a iEFSM" where
   "learn n pta l r m np = (
      let check = accepts_log (set l) in
          (infer {} n pta r m check np)
@@ -618,9 +617,9 @@ outputs can be compared. If a point is reached where the model does not recognis
 remainder of the trace forms the second element of the output pair such that we know the exact point
 at which the model stopped processing.\<close>
 
-definition i_possible_steps :: "iEFSM \<Rightarrow> cfstate \<Rightarrow> registers \<Rightarrow> label \<Rightarrow> inputs \<Rightarrow> (tids \<times> cfstate \<times> transition) fset" where
+definition i_possible_steps :: "('a::aexp_value) iEFSM \<Rightarrow> cfstate \<Rightarrow> 'a registers \<Rightarrow> label \<Rightarrow> 'a inputs \<Rightarrow> (tids \<times> cfstate \<times> 'a transition) fset" where
   "i_possible_steps e s r l i = fimage (\<lambda>(uid, (origin, dest), t). (uid, dest, t))
-  (ffilter (\<lambda>(uid, (origin, dest::nat), t::transition).
+  (ffilter (\<lambda>(uid, (origin, dest), t).
       origin = s
       \<and> (Label t) = l
       \<and> (length i) = (Arity t)
@@ -628,7 +627,7 @@ definition i_possible_steps :: "iEFSM \<Rightarrow> cfstate \<Rightarrow> regist
      )
     e)"
 
-fun test_trace :: "trace \<Rightarrow> iEFSM \<Rightarrow> cfstate \<Rightarrow> registers \<Rightarrow> ((label \<times> inputs \<times> cfstate \<times> cfstate \<times> registers \<times> tids \<times> value list \<times> outputs) list \<times> trace)" where
+fun test_trace :: "('a::aexp_value) trace \<Rightarrow> 'a iEFSM \<Rightarrow> cfstate \<Rightarrow> 'a registers \<Rightarrow> ((label \<times> 'a inputs \<times> cfstate \<times> cfstate \<times> 'a registers \<times> tids \<times> 'a list \<times> 'a outputs) list \<times> 'a trace)" where
   "test_trace [] _ _ _ = ([], [])" |
   "test_trace ((l, i, expected)#es) e s r = (
     let
@@ -646,9 +645,9 @@ fun test_trace :: "trace \<Rightarrow> iEFSM \<Rightarrow> cfstate \<Rightarrow>
         ([], (l, i, expected)#es)
   )"
 
-text\<open>The \texttt{test\_log} function executes the \texttt{test\_trace} function on a collection of
+text\<open>The \texttt{test\_'a log} function executes the \texttt{test\_trace} function on a collection of
 traces known as the \emph{test set.}\<close>
-definition test_log :: "log \<Rightarrow> iEFSM \<Rightarrow> ((label \<times> inputs \<times> cfstate \<times> cfstate \<times> registers \<times> tids \<times> value list \<times> outputs) list \<times> trace) list" where
+definition test_log :: "('a::{aexp_value,order}) log \<Rightarrow> 'a iEFSM \<Rightarrow> ((label \<times> 'a inputs \<times> cfstate \<times> cfstate \<times> 'a registers \<times> tids \<times> 'a list \<times> 'a outputs) list \<times> 'a trace) list" where
   "test_log l e = map (\<lambda>t. test_trace t e 0 <>) l"
 
 end
